HW 10

lean/LoVe/LoVe10_HoareLogic_HomeworkSheet.lean
@@ -22,11 +22,20 @@ The following WHILE program is intended to compute the factorial of `n₀`, leav
 the result in `r`. -/
 
 def FACT : Stmt :=
-  Stmt.assign "i" (fun s ↦ 0);
-  Stmt.assign "r" (fun s ↦ 1);
+  Stmt.assign "i" (fun _ ↦ 0);
+  Stmt.assign "r" (fun _ ↦ 1);
   Stmt.whileDo (fun s ↦ s "i" ≠ s "n")
     (Stmt.assign "i" (fun s ↦ s "i" + 1);
      Stmt.assign "r" (fun s ↦ s "r" * s "i"))
+
+/-
+i := 0
+r := 1
+while i ≠ n do
+  i := i  + 1
+  r := r * i
+end
+-/
 
 /- Recall the definition of the `fact` function: -/
 
@@ -42,9 +51,39 @@ attribute [simp] fact
 Hint: Remember to strengthen the loop invariant with `s "n" = n₀` to
 capture the fact that the variable `n` does not change. -/
 
-theorem FACT_correct (n₀ : ℕ) :
-    {* fun s ↦ s "n" = n₀ *} (FACT) {* fun s ↦ s "r" = fact n₀ *} :=
+lemma natural_number_strictly_smaller {i n: Nat}
+  (leq: i ≤ n) (diff: i ≠ n)
+:
+  i + 1 ≤ n :=
   sorry
+
+
+lemma same_with_inv I:
+  Stmt.whileDo = Stmt.invWhileDo I :=
+    by
+      apply funext
+      intro b
+      apply funext
+      intro C
+      simp [Stmt.invWhileDo]
+
+
+theorem FACT_correct (n₀ : ℕ) :
+    {* fun s ↦ s "n" = n₀ *} (FACT) {* fun s ↦ s "r" = fact n₀ *} := by
+      rw [FACT]
+      rw [same_with_inv (fun s => s "r" = fact (s "i") ∧ s "i" ≤ s "n" ∧ s "n" = n₀)]
+      vcg
+      simp
+      intro s h1 h2 h3 h4
+      apply And.intro _ (And.intro _ h3)
+      rw [h1]
+      ac_rfl
+      exact natural_number_strictly_smaller h2 h4
+      intro s h1 h2
+      have hin: s "i" = s "n" := by
+        aesop
+      simp [h2, hin]
+      simp
 
 
 /- ## Question 2 (5 points + 1 bonus point):
@@ -72,33 +111,61 @@ namespace PartialHoare
 
 theorem consequence {P P' Q Q' S} (h : {* P *} (S) {* Q *})
       (hp : ∀s, P' s → P s) (hq : ∀s, Q s → Q' s) :
-    {* P' *} (S) {* Q' *} :=
-  sorry
+    {* P' *} (S) {* Q' *} := by
+    rw [PartialHoare] at *
+    intro s s' pre trans
+    apply hq s'
+    apply h s
+    apply hp s pre
+    exact trans
 
 theorem assign_intro {P x a} :
     {* fun s ↦ P (s[x ↦ a s]) *} (Stmt.assign x a) {* P *} :=
-  sorry
+    by simp [PartialHoare]
 
 theorem assert_intro {P Q : State → Prop} :
     {* fun s ↦ Q s → P s *} (Stmt.assert Q) {* P *} :=
-  sorry
+    by simp [PartialHoare]
 
 theorem seq_intro {P Q R S T}
       (hS : {* P *} (S) {* Q *}) (hT : {* Q *} (T) {* R *}) :
-    {* P *} (Stmt.seq S T) {* R *} :=
-  sorry
+    {* P *} (Stmt.seq S T) {* R *} := by
+      simp [PartialHoare] at *
+      intro s s' pre s'' trans1 trans2
+      apply hT s''
+      apply hS s
+      exact pre
+      exact trans1
+      exact trans2
+
 
 theorem choice_intro {P Q Ss}
       (h : ∀i (hi : i < List.length Ss), {* P *} (Ss[i]'hi) {* Q *}) :
-    {* P *} (Stmt.choice Ss) {* Q *} :=
-  sorry
+    {* P *} (Stmt.choice Ss) {* Q *} := by
+    simp [PartialHoare] at *
+    intro s s' pre i h_wf trans
+    exact h i _ s _ pre trans
+
 
 /- 2.2 (1 bonus point). Prove the rule for `loop`. Notice the similarity with
 the rule for `while` in the WHILE language. -/
 
 theorem loop_intro {P S} (h : {* P *} (S) {* P *}) :
-    {* P *} (Stmt.loop S) {* P *} :=
-  sorry
+    {* P *} (Stmt.loop S) {* P *} := by
+    rw [PartialHoare] at *
+    intro s s' pre trans
+
+    generalize ws_eq : (S.loop, s) = Ss
+    rw [ws_eq] at trans
+    induction trans generalizing s with
+    | loop_more C s1 s2 s3 hone hloop ih hloop_ih =>
+      apply hloop_ih s2
+      apply h s _ pre
+      aesop
+      aesop
+    | loop_stop => aesop
+    | _ => cases ws_eq
+
 
 end PartialHoare
 
